Lectures/Week08/Sheet3.lean
@@ -30,22 +30,45 @@ set_option tactic.hygienic false
         grind
 
 @[simp] theorem merge_ret_length_eq_sum (xs ys : List ℕ) :
-  (merge xs ys).ret.length = xs.length + ys.length := by sorry
+  (merge xs ys).ret.length = xs.length + ys.length := by
+ match  xs, ys with
+ | [], x => simp [merge, merge.go]
+ | xs, [] =>
+   unfold merge merge.go
+   aesop -- why `grind` does not solve it?
+ | a :: as, b :: bs =>
+   simp +arith +decide only [List.length_cons, merge, merge.go]
+   split_ifs
+   · simp
+     rw [← merge]
+     apply merge_ret_length_eq_sum
+   · simp
+     rw [← merge]
+     -- rw [merge_ret_length_eq_sum]
+     -- simp ; linarith
+     -- it looks like tail recursive of the theorem is relevant here?
+     rw [Nat.add_assoc, Nat.add_comm _ 1, ← Nat.add_assoc]
+     apply merge_ret_length_eq_sum
 
 @[simp] theorem mergeSort_same_length (xs : List ℕ) :
-  (mergeSort xs).ret.length = xs.length:= by sorry
+  (mergeSort xs).ret.length = xs.length:= by
+  unfold mergeSort
+  split
+  next h =>
+   simp
+  next h =>
+   simp
+   repeat rw [mergeSort_same_length]
+   grind only [= List.length_drop, = List.length_take, = min_def]
+
 
 -- Next, we pave our way towards proving O(n log n) running time of merge sort.
 
-example (xs : List ℕ) (h : ∃ k, xs.length = 2 ^ k) :
-  (mergeSort xs).time = xs.length*(Nat.log 2 xs.length)  := by sorry
-
 def MS_REC : ℕ → ℕ
 | 0 => 0
-| n@(x+1) =>
-  if x = 0 then 0
-  else
-    MS_REC (n/2) + MS_REC ((n-1)/2 + 1) + n
+| 1 => 0
+| n@(_x + 2) =>
+  MS_REC (n / 2) + MS_REC ((n - 1)/2 + 1) + n
 
 #eval mergeSort [4,1,3,4,5,6]
 #eval MS_REC 10
@@ -53,66 +76,32 @@ def MS_REC : ℕ → ℕ
 theorem mergeSort_time_eq_MS_REC (xs : List ℕ) :
   (mergeSort xs).time = MS_REC xs.length := by
   fun_induction mergeSort
-  · simp only [Pure.pure, pure]
+  · simp only [TimeM.tick]
     unfold MS_REC
-    simp_all
     grind
-  · simp_all only [not_lt, Bind.bind, TimeM.time_of_bind, merge_time, mergeSort_same_length]
-    conv =>
-      right
-      unfold MS_REC
-    simp_all
-    split
-    · simp_all
-    · simp_all
-      grind
+  · simp only [bind, TimeM.time_of_bind, merge_time, mergeSort_same_length]
+    unfold MS_REC
+    grind
 
 def MS_REC_SIMP : ℕ → ℕ
 | 0 => 0
-| n@(x+1) =>
-  if x = 0 then 0
-  else
-    2*MS_REC_SIMP (n/2) + n
+| 1 => 0
+| n@(_x + 1) =>
+  2 * MS_REC_SIMP (n / 2) + n
+
 
 theorem MS_REC_SIMP_EQ (n : ℕ)
   : (MS_REC (2^n)) = (MS_REC_SIMP (2^n))  := by
   induction' n  with n ih
   · unfold MS_REC_SIMP MS_REC
-    simp only [↓reduceIte]
+    rfl
   · unfold MS_REC_SIMP MS_REC
-    split <;> all_goals (simp_all)
-    rename_i heq
-    split
-    next h =>
-      subst h
-      simp_all only [zero_add, Nat.pow_eq_one, OfNat.ofNat_ne_one]
-    next h =>
-      simp_all only [Nat.add_right_cancel_iff]
-      rw [← heq]
-      grind
-
+    grind
 
 theorem MS_REC_SIMP_EQ_CLOSED (n : ℕ) : MS_REC_SIMP (2^n) = 2^n * n := by
-  induction' n  with n ih
-  · unfold MS_REC_SIMP
-    aesop
-  · unfold MS_REC_SIMP
-    simp_all only
-    split
-    next heq =>
-      simp_all only [Nat.pow_eq_zero, OfNat.ofNat_ne_zero, ne_eq,
-        Nat.add_eq_zero_iff, one_ne_zero, and_false, not_false_eq_true,
-        and_true]
-    next heq =>
-      simp_all only [Nat.succ_eq_add_one]
-      split
-      next h =>
-        subst h
-        simp_all only [zero_add, Nat.pow_eq_one, OfNat.ofNat_ne_one,
-          Nat.add_eq_zero_iff, one_ne_zero, and_false, or_self]
-      next h =>
-        rw [← heq]
-        grind
+  induction' n with n ih
+  all_goals unfold MS_REC_SIMP ; grind
+
 
 -- The time is written assuming the length of the list is a power of two (for simplicity).
 theorem MStimeBound (xs : List ℕ) (h : ∃ k, xs.length = 2 ^ k) :
